decomposed WF_flat into 2 lemmas

SemLab/AFlatCont.v
@@ -17,6 +17,7 @@ Require Import SN.
 Require Import EqUtil.
 Require Import VecUtil.
 Require Import Max.
+Require Import RelUtil.
 
 (***********************************************************************)
 (** flat context closure for standard rewriting *)
@@ -82,17 +83,14 @@ Variable hyp : arity some_symbol > 0.
 
 Definition one_flat_cont := flat_cont_symb n some_symbol hyp.
 
-Lemma WF_flat : WF (red R) <-> WF (red R').
+Lemma red_flat : red R' << red R.
 
 Proof.
-split; intro.
-(* -> *)
-intro t. generalize (H t). induction 1. apply SN_intro; intros. apply H1.
-redtac. unfold flat_rules in lr. rewrite in_flat_map in lr.
+intros t u h. redtac. unfold flat_rules in lr. rewrite in_flat_map in lr.
 destruct lr as [[a b] [h1 h2]]. unfold flat_rule in h2. simpl in h2.
-destruct a. simpl in h2. intuition. inversion H2. subst. apply red_rule. hyp.
-destruct b. simpl in h2. intuition. inversion H2. subst. apply red_rule. hyp.
-gen h2. case_symb_eq Sig f f0; intro. simpl in h2. intuition. inversion H2.
+destruct a. simpl in h2. intuition. inversion H. subst. apply red_rule. hyp.
+destruct b. simpl in h2. intuition. inversion H. subst. apply red_rule. hyp.
+gen h2. case_symb_eq Sig f f0; intro. simpl in h2. intuition. inversion H.
 subst. apply red_rule. hyp. rewrite in_map_iff in h2.
 destruct h2 as [d [h3 h4]]. unfold flat_cont_rule in h3. inversion h3.
 clear h3. subst. unfold flat_conts in h4. rewrite in_flat_map in h4.
@@ -106,16 +104,22 @@ set (v' := Vmap (sub s) v). set (v0' := Vmap (sub s) v0).
 change (red R (fill c (fill d' (sub s (Fun f v))))
            (fill c (fill d' (sub s (Fun f0 v0))))). repeat rewrite fill_fill.
 apply red_rule. hyp.
-(* <- *)
-intro t. geneq H t (fill one_flat_cont t). induction 1. intros. subst.
-apply SN_intro; intros. apply H0 with (fill one_flat_cont y). 2: refl.
-redtac. subst. repeat rewrite fill_fill.
+Qed.
+
+Definition red_one_flat_cont := Rof (red R') (fill one_flat_cont).
+
+Notation redR'c := red_one_flat_cont.
+ 
+Lemma red_one_flat_cont_intro : red R << redR'c.
+
+Proof.
+intros t u h. redtac. subst. unfold redR'c, Rof. repeat rewrite fill_fill.
 case_eq (is_root_preserving (mkRule l r)). apply red_rule.
 unfold flat_rules. rewrite in_flat_map.
-exists (mkRule l r). intuition. unfold flat_rule. rewrite H1. simpl. auto.
+exists (mkRule l r). intuition. unfold flat_rule. rewrite H. simpl. auto.
 destruct l. discr. destruct r. discr.
 destruct (cont_case (comp one_flat_cont c)). discr.
-destruct H2 as [d [g [i [vi [j [vj [e]]]]]]]. repeat rewrite H2.
+destruct H0 as [d [g [i [vi [j [vj [e]]]]]]]. repeat rewrite H0.
 repeat rewrite <- fill_fill. set (l := Fun f v). set (r := Fun f0 v0).
 apply context_closed_red.
 assert (m : maxvar_rule (mkRule l r) < S n). eapply maxvar_rules_elim.
@@ -124,15 +128,28 @@ repeat rewrite fill_sub with (n:=n).
 set (s' := maxvar_union (S n) s (fsub n (Vapp vi vj))).
 apply hd_red_incl_red. apply hd_red_rule. unfold flat_rules.
 rewrite in_flat_map. exists (mkRule l r). intuition. unfold flat_rule.
-unfold l, r. rewrite H1. rewrite in_map_iff. assert (h : i < arity g). omega.
+unfold l, r. rewrite H. rewrite in_map_iff. assert (h : i < arity g). omega.
 exists (flat_cont_symb (S n) g h). intuition. simpl.
-generalize (flat_cont_aux h). assert (arity g - S i = j). omega. rewrite H3.
+generalize (flat_cont_aux h). assert (arity g - S i = j). omega. rewrite H1.
 intro. assert (e0=e). apply eq_unique. subst. refl.
 unfold flat_conts. rewrite in_flat_map. exists g. split. apply Fs_ok.
 unfold flat_conts_symb. rewrite in_map_iff. exists (mk_nat_lt h). intuition.
 apply nats_lt_complete.
 transitivity (maxvar_rule (mkRule l r)). omega. apply le_max_r.
 transitivity (maxvar_rule (mkRule l r)). omega. apply le_max_l.
+Qed.
+
+Lemma WF_flat : WF (red R) <-> WF (red R').
+
+Proof.
+split; intro.
+(* -> *)
+intro t. generalize (H t). induction 1. apply SN_intro; intros. apply H1.
+apply red_flat. hyp.
+(* <- *)
+intro t. geneq H t (fill one_flat_cont t). induction 1. intros. subst.
+apply SN_intro; intros. apply H0 with (fill one_flat_cont y). 2: refl.
+apply red_one_flat_cont_intro. hyp.
 Qed.
 
 End S.
